Utils.thy
@@ -1,0 +1,84 @@
+theory Utils imports Syntax begin
+
+free_constructors packet for PktIn | PktOut
+using packet.strong_exhaust apply auto done
+(* TODO: Are these warnings bad? Can I do something about them? *)
+(* TODO: Is it preferable to do this, or make every function matching on packets
+         a nominal_function? *)
+(* TODO: This works when done here but not when done in Syntax? *)
+
+fun slice :: "'a list \<Rightarrow> int \<Rightarrow> int \<Rightarrow> 'a list" where
+  "slice xs n m = take (nat (m - n)) (drop (nat n) xs)"
+
+text\<open>Replaces [n:m) in the first input list with the second list.\<close>
+fun splice :: "'a list \<Rightarrow> int \<Rightarrow> int \<Rightarrow> 'a list \<Rightarrow> 'a list" where
+  "splice xs n m ins = (slice xs 0 n) @ ins @ (slice xs m (int (length xs)))"
+
+section\<open>Headers\<close>
+
+text\<open>This is necessary to use headers (and heaps later)  in nominal_functions. It basically states
+that no variables actually appear in the type.\<close>
+instantiation headers :: pure begin
+  definition permute_headers :: "perm \<Rightarrow> headers \<Rightarrow> headers" where
+    "permute_headers _ x = x"
+  instance by standard (auto simp add: permute_headers_def)
+end
+
+definition "empty_headers = Headers Map.empty"
+
+fun header_lookup :: "headers \<Rightarrow> instanc \<Rightarrow> bv option" where
+  "header_lookup (Headers h) i = h i" 
+
+fun header_update :: "headers \<Rightarrow> instanc \<Rightarrow> bv \<Rightarrow> headers" where
+  "header_update (Headers h) i bs = Headers (h(i := Some bs))"
+
+thm map_update
+
+fun header_field_to_range_helper :: "int \<Rightarrow> field list \<Rightarrow> field_name \<Rightarrow> (int \<times> int)" where
+  "header_field_to_range_helper acc ((Field fn fl)#fs) tgt = (if fn = tgt then (acc, acc + fl)
+    else header_field_to_range_helper (acc + fl) fs tgt)" |
+  "header_field_to_range_helper acc [] tgt = undefined"
+
+fun header_field_to_range :: "header_type \<Rightarrow> field_name \<Rightarrow> (int \<times> int)" where
+  "header_field_to_range (HeaderType _ fs) tgt = header_field_to_range_helper 0 fs tgt"
+
+section\<open>Heaps and Envs\<close>
+
+instantiation heap :: pure begin
+  definition permute_heap :: "perm \<Rightarrow> heap \<Rightarrow> heap"  where
+    "permute_heap _ x = x"
+  instance by standard (auto simp add: permute_heap_def)
+end
+
+fun triple_to_heap :: "bv \<Rightarrow> bv \<Rightarrow> headers \<Rightarrow> heap" where
+  "triple_to_heap In Out H = Heap In Out H"
+
+fun heap_lookup_packet :: "heap \<Rightarrow> packet \<Rightarrow> bv" where
+  "heap_lookup_packet (Heap In Out _) PktIn = In" |
+  "heap_lookup_packet (Heap In Out _) PktOut = Out"
+
+fun heap_lookup_instance :: "heap \<Rightarrow> instanc \<Rightarrow> bv option" where
+  "heap_lookup_instance (Heap _ _ (Headers insts)) i = insts i"
+
+(* Easier to work with than "var \<Rightarrow> heap" with Nominal2 because it has a finite support (I think) *)
+type_synonym env = "(var \<times> heap) list"
+
+fun env_lookup_packet :: "env \<Rightarrow> var \<Rightarrow> packet \<Rightarrow> bv option" where
+  "env_lookup_packet \<epsilon> x p = map_option (\<lambda>h. heap_lookup_packet h p) (map_of \<epsilon> x)"
+fun env_lookup_instance :: "env \<Rightarrow> var \<Rightarrow> instanc \<Rightarrow> bv option" where
+  "env_lookup_instance \<epsilon> x i = Option.bind (map_of \<epsilon> x) (\<lambda>h. heap_lookup_instance h i)"
+nominal_function env_lookup_sliceable :: "env \<Rightarrow> sliceable \<Rightarrow> bv option" where
+  "env_lookup_sliceable \<epsilon> (SlPacket x p) = env_lookup_packet \<epsilon> x p" |
+  "env_lookup_sliceable \<epsilon> (SlInstance x i) = env_lookup_instance \<epsilon> x i"
+  (*using [[simproc del: alpha_lst defined_all]]*)
+  subgoal by (simp add: eqvt_def env_lookup_sliceable_graph_aux_def)
+  subgoal by (erule env_lookup_sliceable_graph.induct) (auto)
+  apply clarify
+  subgoal for P e s
+    by (rule sliceable.strong_exhaust[of s P]) (auto)
+  apply (simp_all)
+done
+nominal_termination (eqvt)
+  by lexicographic_order
+
+end
